src/Specific/IntegrationTestTemporaryMiscCommon.v
@@ -1,6 +1,12 @@
 (*** XXX TODO MOVE ALL THINGS IN THIS FILE TO BETTER PLACES *)
+Require Import Coq.ZArith.BinInt.
 Require Import Coq.Classes.Morphisms.
 Require Import Crypto.Util.Tuple.
+Require Import Crypto.Util.Sigma.Lift.
+Require Import Crypto.Util.Sigma.Associativity.
+Require Import Crypto.Util.Sigma.MapProjections.
+Require Import Crypto.Util.Tactics.MoveLetIn.
+Require Import Crypto.Util.Tactics.DestructHead.
 
 Definition adjust_tuple2_tuple2_sig {A P Q}
            (v : { a : { a : tuple (tuple A 2) 2 | (P (fst (fst a)) /\ P (snd (fst a))) /\ (P (fst (snd a)) /\ P (snd (snd a))) }
@@ -78,3 +84,113 @@ Definition sig_conj_by_impl2 {A} {P Q : A -> Prop} (H : forall a : A, Q a -> P a
            (H' : { a : A | Q a })
   : { a : A | P a /\ Q a }
   := let (a, p) := H' in exist _ a (conj (H a p) p).
+
+
+(** [apply_lift_sig] picks out which version of the [liftN_sig] lemma
+    to apply, and builds the appropriate arguments *)
+Ltac make_P_for_apply_lift_sig P :=
+  lazymatch P with
+  | fun (f : ?F) => forall (a : ?A), @?P f a
+    => constr:(fun (a : A)
+               => ltac:(lazymatch constr:(fun (f : F)
+                                          => ltac:(let v := (eval cbv beta in (P f a)) in
+                                                   lazymatch (eval pattern (f a) in v) with
+                                                   | ?k _ => exact k
+                                                   end))
+                        with
+                        | fun _ => ?P
+                          => let v := make_P_for_apply_lift_sig P in
+                             exact v
+                        end))
+  | _ => P
+  end.
+Ltac apply_lift_sig :=
+  let P := lazymatch goal with |- sig ?P => P end in
+  let P := make_P_for_apply_lift_sig P in
+  lazymatch goal with
+  | [ |- { f | forall a b c d e, _ } ]
+    => fail "apply_lift_sig does not yet support ≥ 5 binders"
+  | [ |- { f | forall (a : ?A) (b : ?B) (c : ?C) (d : ?D), _ } ]
+    => apply (@lift4_sig A B C D _ P)
+  | [ |- { f | forall (a : ?A) (b : ?B) (c : ?C), _ } ]
+    => apply (@lift3_sig A B C _ P)
+  | [ |- { f | forall (a : ?A) (b : ?B), _ } ]
+    => apply (@lift2_sig A B _ P)
+  | [ |- { f | forall (a : ?A), _ } ]
+    => apply (@lift1_sig A _ P)
+  | [ |- { f | _ } ]
+    => idtac
+  end.
+Ltac start_preglue :=
+  apply_lift_sig; intros;
+  let phi := lazymatch goal with |- { f | ?phi _ = _ } => phi end in
+  eexists_sig_etransitivity; cbv [phi].
+Ltac do_set_sig f_sig :=
+  let fZ := fresh f_sig in
+  set (fZ := proj1_sig f_sig);
+  context_to_dlet_in_rhs fZ; cbv beta delta [fZ];
+  try cbv beta iota delta [proj1_sig f_sig];
+  cbv beta iota delta [fst snd].
+Ltac do_rewrite_with_sig_by f_sig by_tac :=
+  let lem := constr:(proj2_sig f_sig) in
+  let lemT := type of lem in
+  let lemT := (eval cbv beta zeta in lemT) in
+  rewrite <- (lem : lemT) by by_tac ();
+  do_set_sig f_sig.
+Ltac do_rewrite_with_sig f_sig := do_rewrite_with_sig_by f_sig ltac:(fun _ => idtac).
+Ltac do_rewrite_with_1sig_add_carry_by f_sig carry_sig by_tac :=
+  let fZ := fresh f_sig in
+  rewrite <- (proj2_sig f_sig) by by_tac ();
+  symmetry; rewrite <- (proj2_sig carry_sig) by by_tac (); symmetry;
+  pose (fun a => proj1_sig carry_sig (proj1_sig f_sig a)) as fZ;
+  lazymatch goal with
+  | [ |- context G[proj1_sig carry_sig (proj1_sig f_sig ?a)] ]
+    => let G' := context G[fZ a] in change G'
+  end;
+  context_to_dlet_in_rhs fZ; cbv beta delta [fZ];
+  try cbv beta iota delta [proj1_sig f_sig carry_sig];
+  cbv beta iota delta [fst snd].
+Ltac do_rewrite_with_1sig_add_carry f_sig carry_sig := do_rewrite_with_1sig_add_carry_by f_sig carry_sig ltac:(fun _ => idtac).
+Ltac do_rewrite_with_2sig_add_carry_by f_sig carry_sig by_tac :=
+  let fZ := fresh f_sig in
+  rewrite <- (proj2_sig f_sig) by by_tac ();
+  symmetry; rewrite <- (proj2_sig carry_sig) by by_tac (); symmetry;
+  pose (fun a b => proj1_sig carry_sig (proj1_sig f_sig a b)) as fZ;
+  lazymatch goal with
+  | [ |- context G[proj1_sig carry_sig (proj1_sig f_sig ?a ?b)] ]
+    => let G' := context G[fZ a b] in change G'
+  end;
+  context_to_dlet_in_rhs fZ; cbv beta delta [fZ];
+  try cbv beta iota delta [proj1_sig f_sig carry_sig];
+  cbv beta iota delta [fst snd].
+Ltac do_rewrite_with_2sig_add_carry f_sig carry_sig := do_rewrite_with_2sig_add_carry_by f_sig carry_sig ltac:(fun _ => idtac).
+Ltac fin_preglue :=
+  [ > reflexivity
+  | repeat sig_dlet_in_rhs_to_context;
+    apply (fun f => proj2_sig_map (fun THIS_NAME_MUST_NOT_BE_UNDERSCORE_TO_WORK_AROUND_CONSTR_MATCHING_ANAOMLIES___BUT_NOTE_THAT_IF_THIS_NAME_IS_LOWERCASE_A___THEN_REIFICATION_STACK_OVERFLOWS___AND_I_HAVE_NO_IDEA_WHATS_GOING_ON p => f_equal f p)) ].
+
+Ltac factor_out_bounds_and_strip_eval op_bounded op_sig_side_conditions_t :=
+  let feBW_small := lazymatch goal with |- { f : ?feBW_small | _ } => feBW_small end in
+  Associativity.sig_sig_assoc;
+  apply sig_conj_by_impl2;
+  [ let H := fresh in
+    intros ? H;
+    try lazymatch goal with
+        | [ |- (?eval _ < _)%Z ]
+          => cbv [eval]
+        end;
+    rewrite H; clear H;
+    eapply Z.le_lt_trans;
+      [ apply Z.eq_le_incl, f_equal | apply op_bounded ];
+      [ repeat match goal with
+               | [ |- ?f ?x = ?g ?y ]
+                 => is_evar y; unify x y;
+                    apply (f_equal (fun fg => fg x))
+               end;
+        clear; abstract reflexivity
+      | .. ];
+      op_sig_side_conditions_t ()
+  | apply (fun f => proj2_sig_map (fun THIS_NAME_MUST_NOT_BE_UNDERSCORE_TO_WORK_AROUND_CONSTR_MATCHING_ANAOMLIES___BUT_NOTE_THAT_IF_THIS_NAME_IS_LOWERCASE_A___THEN_REIFICATION_STACK_OVERFLOWS___AND_I_HAVE_NO_IDEA_WHATS_GOING_ON p => f_equal f p));
+    repeat match goal with
+           | [ H : feBW_small |- _ ] => destruct H as [? _]
+           end ].
